update

Coq/Coq29.v
@@ -1,3 +1,8 @@
+(*
+  Exercises for <Software Foundations> V2 CH5.
+  Author : Brethland, Late 2019.
+*)
+
 Set Warnings "-notation-overridden,-parsing".
 From Coq Require Import Arith.Arith.
 From Coq Require Import Arith.EqNat.
@@ -346,3 +351,343 @@ Proof.
       apply H. apply H0. subst. apply (IHP11 P12 y2) in H1.
       auto. auto.
 Qed.
+
+Lemma multistep_congr_2 : ∀t1 t2 t2',
+     value t1 →
+     t2 -->* t2' →
+     P t1 t2 -->* P t1 t2'.
+Proof.
+  intros. induction H0;try constructor.
+  apply multi_step with (P t1 y). econstructor;auto. auto.
+Qed.
+
+Lemma multistep_congr_1 : ∀t1 t1' t2,
+     t1 -->* t1' →
+     P t1 t2 -->* P t1' t2.
+Proof.
+  intros t1 t1' t2 H. induction H.
+  - (* multi_refl *) apply multi_refl.
+  - (* multi_step *) apply multi_step with (P y t2).
+    + apply ST_Plus1. apply H.
+    + apply IHmulti.
+Qed.
+
+Theorem step_normalizing :
+  normalizing step.
+Proof.
+  unfold normalizing.
+  induction t.
+  - exists (C n).
+    split.
+    + apply multi_refl.
+    + rewrite nf_same_as_value. apply v_const.
+  - destruct IHt1 as [t1' [Hsteps1 Hnormal1]].
+    destruct IHt2 as [t2' [Hsteps2 Hnormal2]].
+    rewrite nf_same_as_value in Hnormal1.
+    rewrite nf_same_as_value in Hnormal2.
+    inversion Hnormal1 as [n1 H1].
+    inversion Hnormal2 as [n2 H2].
+    rewrite <- H1 in Hsteps1.
+    rewrite <- H2 in Hsteps2.
+    exists (C (n1 + n2)).
+    split.
+    + apply multi_trans with (P (C n1) t2).
+      * apply multistep_congr_1. apply Hsteps1.
+      * apply multi_trans with
+        (P (C n1) (C n2)).
+        { apply multistep_congr_2. apply v_const. apply Hsteps2. }
+        apply multi_R. { apply ST_PlusConstConst. }
+    + rewrite nf_same_as_value. apply v_const.
+Qed.
+
+Theorem eval__multistep : ∀t n,
+  t ===> n → t -->* C n.
+Proof.
+  intros. induction H;try constructor.
+  assert (P t1 t2 -->* P (C n1) t2).
+  apply multistep_congr_1. auto.
+  apply multi_trans with (P (C n1) t2). auto.
+  assert (P (C n1) t2 -->* P (C n1) (C n2)).
+  apply multistep_congr_2. constructor. auto.
+  apply multi_trans with (P (C n1) (C n2)). auto.
+  apply multi_R. constructor.
+Qed.
+
+Lemma step__eval : ∀t t' n,
+     t ---> t' →
+     t' ===> n →
+     t ===> n.
+Proof.
+  intros t t' n Hs. generalize dependent n.
+  induction Hs;intros.
+  - inversion H. constructor;constructor.
+  - inversion H;subst. apply (IHHs (n1)) in H2.
+    constructor;auto.
+  - inversion H0;subst. apply (IHHs (n2)) in H5.
+    constructor;auto.
+Qed.
+
+Theorem multistep__eval : ∀t t',
+  normal_form_of t t' → ∃n, t' = C n ∧ t ===> n.
+Proof.
+  intros. unfold normal_form_of in H. destruct H.
+  unfold step_normal_form in H0. apply nf_same_as_value in H0.
+  inversion H0. exists n. split. auto. induction H;subst. constructor.
+  apply step__eval with y. auto. apply IHmulti. auto. auto.
+Qed.
+
+Theorem evalF_eval : ∀t n,
+  evalF t = n ↔ t ===> n.
+Proof.
+  split.
+  - generalize dependent n. induction t;intros.
+    simpl in H;subst;constructor.
+    simpl in H. remember (evalF t1) as n1. remember (evalF t2) as n2.
+    specialize (IHt1 n1). specialize (IHt2 n2). 
+    rewrite <- H. constructor. apply IHt1. auto. apply IHt2. auto.
+  - intros. induction H. simpl. auto.
+    simpl. subst. auto.
+Qed.
+
+Inductive aval : aexp → Prop :=
+  | av_num : ∀n, aval (ANum n).
+
+Reserved Notation " t '/' st '-->a' t' "
+                  (at level 40, st at level 39).
+Inductive astep : state → aexp → aexp → Prop :=
+  | AS_Id : ∀st i,
+      AId i / st -->a ANum (st i)
+  | AS_Plus1 : ∀st a1 a1' a2,
+      a1 / st -->a a1' →
+      (APlus a1 a2) / st -->a (APlus a1' a2)
+  | AS_Plus2 : ∀st v1 a2 a2',
+      aval v1 →
+      a2 / st -->a a2' →
+      (APlus v1 a2) / st -->a (APlus v1 a2')
+  | AS_Plus : ∀st n1 n2,
+      APlus (ANum n1) (ANum n2) / st -->a ANum (n1 + n2)
+  | AS_Minus1 : ∀st a1 a1' a2,
+      a1 / st -->a a1' →
+      (AMinus a1 a2) / st -->a (AMinus a1' a2)
+  | AS_Minus2 : ∀st v1 a2 a2',
+      aval v1 →
+      a2 / st -->a a2' →
+      (AMinus v1 a2) / st -->a (AMinus v1 a2')
+  | AS_Minus : ∀st n1 n2,
+      (AMinus (ANum n1) (ANum n2)) / st -->a (ANum (minus n1 n2))
+  | AS_Mult1 : ∀st a1 a1' a2,
+      a1 / st -->a a1' →
+      (AMult a1 a2) / st -->a (AMult a1' a2)
+  | AS_Mult2 : ∀st v1 a2 a2',
+      aval v1 →
+      a2 / st -->a a2' →
+      (AMult v1 a2) / st -->a (AMult v1 a2')
+  | AS_Mult : ∀st n1 n2,
+      (AMult (ANum n1) (ANum n2)) / st -->a (ANum (mult n1 n2))
+
+    where " t '/' st '-->a' t' " := (astep st t t').
+Reserved Notation " t '/' st '-->b' t' "
+                  (at level 40, st at level 39).
+Inductive bstep : state → bexp → bexp → Prop :=
+| BS_Eq1 : ∀st a1 a1' a2,
+    a1 / st -->a a1' →
+    (BEq a1 a2) / st -->b (BEq a1' a2)
+| BS_Eq2 : ∀st v1 a2 a2',
+    aval v1 →
+    a2 / st -->a a2' →
+    (BEq v1 a2) / st -->b (BEq v1 a2')
+| BS_Eq : ∀st n1 n2,
+    (BEq (ANum n1) (ANum n2)) / st -->b
+    (if (n1 =? n2) then BTrue else BFalse)
+| BS_LtEq1 : ∀st a1 a1' a2,
+    a1 / st -->a a1' →
+    (BLe a1 a2) / st -->b (BLe a1' a2)
+| BS_LtEq2 : ∀st v1 a2 a2',
+    aval v1 →
+    a2 / st -->a a2' →
+    (BLe v1 a2) / st -->b (BLe v1 a2')
+| BS_LtEq : ∀st n1 n2,
+    (BLe (ANum n1) (ANum n2)) / st -->b
+             (if (n1 <=? n2) then BTrue else BFalse)
+| BS_NotStep : ∀st b1 b1',
+    b1 / st -->b b1' →
+    (BNot b1) / st -->b (BNot b1')
+| BS_NotTrue : ∀st,
+    (BNot BTrue) / st -->b BFalse
+| BS_NotFalse : ∀st,
+    (BNot BFalse) / st -->b BTrue
+| BS_AndTrueStep : ∀st b2 b2',
+    b2 / st -->b b2' →
+    (BAnd BTrue b2) / st -->b (BAnd BTrue b2')
+| BS_AndStep : ∀st b1 b1' b2,
+    b1 / st -->b b1' →
+    (BAnd b1 b2) / st -->b (BAnd b1' b2)
+| BS_AndTrueTrue : ∀st,
+    (BAnd BTrue BTrue) / st -->b BTrue
+| BS_AndTrueFalse : ∀st,
+    (BAnd BTrue BFalse) / st -->b BFalse
+| BS_AndFalse : ∀st b2,
+    (BAnd BFalse b2) / st -->b BFalse
+
+where " t '/' st '-->b' t' " := (bstep st t t').
+
+Reserved Notation " t '/' st '-->' t' '/' st' "
+                  (at level 40, st at level 39, t' at level 39).
+Open Scope imp_scope.
+Inductive cstep : (com * state) → (com * state) → Prop :=
+  | CS_AssStep : ∀st i a a',
+      a / st -->a a' →
+      (i ::= a) / st --> (i ::= a') / st
+  | CS_Ass : ∀st i n,
+      (i ::= (ANum n)) / st --> SKIP / (i !-> n ; st)
+  | CS_SeqStep : ∀st c1 c1' st' c2,
+      c1 / st --> c1' / st' →
+      (c1 ;; c2) / st --> (c1' ;; c2) / st'
+  | CS_SeqFinish : ∀st c2,
+      (SKIP ;; c2) / st --> c2 / st
+  | CS_IfStep : ∀st b b' c1 c2,
+      b / st -->b b' →
+      IFB b THEN c1 ELSE c2 FI / st
+      -->
+      (IFB b' THEN c1 ELSE c2 FI) / st
+  | CS_IfTrue : ∀st c1 c2,
+      IFB BTrue THEN c1 ELSE c2 FI / st --> c1 / st
+  | CS_IfFalse : ∀st c1 c2,
+      IFB BFalse THEN c1 ELSE c2 FI / st --> c2 / st
+  | CS_While : ∀st b c1,
+      WHILE b DO c1 END / st
+      -->
+      (IFB b THEN c1;; WHILE b DO c1 END ELSE SKIP FI) / st
+
+  where " t '/' st '-->' t' '/' st' " := (cstep (t,st) (t',st')).
+Close Scope imp_scope.
+
+Module CImp.
+Inductive com : Type :=
+  | CSkip : com
+  | CAss : string → aexp → com
+  | CSeq : com → com → com
+  | CIf : bexp → com → com → com
+  | CWhile : bexp → com → com
+  | CPar : com → com → com. (* <--- NEW *)
+Notation "'SKIP'" :=
+  CSkip.
+Notation "x '::=' a" :=
+  (CAss x a) (at level 60).
+Notation "c1 ;; c2" :=
+  (CSeq c1 c2) (at level 80, right associativity).
+Notation "'WHILE' b 'DO' c 'END'" :=
+  (CWhile b c) (at level 80, right associativity).
+Notation "'TEST' b 'THEN' c1 'ELSE' c2 'FI'" :=
+  (CIf b c1 c2) (at level 80, right associativity).
+Notation "'PAR' c1 'WITH' c2 'END'" :=
+  (CPar c1 c2) (at level 80, right associativity).
+Inductive cstep : (com * state) → (com * state) → Prop :=
+    (* Old part *)
+  | CS_AssStep : ∀st i a a',
+      a / st -->a a' →
+      (i ::= a) / st --> (i ::= a') / st
+  | CS_Ass : ∀st i n,
+      (i ::= (ANum n)) / st --> SKIP / (i !-> n ; st)
+  | CS_SeqStep : ∀st c1 c1' st' c2,
+      c1 / st --> c1' / st' →
+      (c1 ;; c2) / st --> (c1' ;; c2) / st'
+  | CS_SeqFinish : ∀st c2,
+      (SKIP ;; c2) / st --> c2 / st
+  | CS_IfStep : ∀st b b' c1 c2,
+      b /st -->b b' →
+          (TEST b THEN c1 ELSE c2 FI) / st
+      --> (TEST b' THEN c1 ELSE c2 FI) / st
+  | CS_IfTrue : ∀st c1 c2,
+      (TEST BTrue THEN c1 ELSE c2 FI) / st --> c1 / st
+  | CS_IfFalse : ∀st c1 c2,
+      (TEST BFalse THEN c1 ELSE c2 FI) / st --> c2 / st
+  | CS_While : ∀st b c1,
+          (WHILE b DO c1 END) / st
+      --> (TEST b THEN (c1;; (WHILE b DO c1 END)) ELSE SKIP FI) / st
+    (* New part: *)
+  | CS_Par1 : ∀st c1 c1' c2 st',
+      c1 / st --> c1' / st' →
+      (PAR c1 WITH c2 END) / st --> (PAR c1' WITH c2 END) / st'
+  | CS_Par2 : ∀st c1 c2 c2' st',
+      c2 / st --> c2' / st' →
+      (PAR c1 WITH c2 END) / st --> (PAR c1 WITH c2' END) / st'
+  | CS_ParDone : ∀st,
+      (PAR SKIP WITH SKIP END) / st --> SKIP / st
+  where " t '/' st '-->' t' '/' st' " := (cstep (t,st) (t',st')).
+Definition cmultistep := multi cstep.
+Notation " t '/' st '-->*' t' '/' st' " :=
+   (multi cstep (t,st) (t',st'))
+   (at level 40, st at level 39, t' at level 39).
+
+Definition par_loop : com :=
+  PAR
+    Y ::= 1
+  WITH
+    WHILE Y = 0 DO
+      X ::= X + 1
+    END
+  END.
+
+Lemma par_body_n__Sn : ∀n st,
+  st X = n ∧ st Y = 0 →
+  par_loop / st -->* par_loop / (X !-> S n ; st).
+Proof.
+  intros. eapply multi_step.
+  apply CS_Par2. apply CS_While.
+  eapply multi_step.
+  apply CS_Par2. apply CS_IfStep.
+  apply BS_Eq1. apply AS_Id.
+  eapply multi_step. apply CS_Par2.
+  apply CS_IfStep. apply BS_Eq.
+  simpl. eapply multi_step.
+  destruct H. assert (st Y =? 0 = true). apply beq_nat_true_iff. auto.
+  rewrite H. apply CS_Par2. apply CS_IfTrue.
+  eapply multi_step. apply CS_Par2. apply CS_SeqStep. apply CS_AssStep.
+  apply AS_Plus1. apply AS_Id.
+  eapply multi_step. apply CS_Par2. apply CS_SeqStep. apply CS_AssStep.
+  destruct H. rewrite e. apply AS_Plus.
+  eapply multi_step. apply CS_Par2. apply CS_SeqStep. apply CS_Ass.
+  eapply multi_step. apply CS_Par2. apply CS_SeqFinish.
+  unfold par_loop. replace (n + 1) with (S n). apply multi_refl.
+  omega.
+Qed.
+
+Lemma par_body_n : ∀n st,
+  st X = 0 ∧ st Y = 0 →
+  ∃st',
+    par_loop / st -->* par_loop / st' ∧ st' X = n ∧ st' Y = 0.
+Proof.
+  intros. induction n.
+  - exists st. split. apply multi_refl. auto.
+  - destruct IHn. destruct H0. exists (X !-> S n ; x). split.
+    eapply multi_trans. apply H0. apply par_body_n__Sn. auto.
+    unfold t_update. simpl. split. auto. destruct H1. auto.
+Qed.
+
+End CImp.
+
+Definition stack := list nat.
+Definition prog := list sinstr.
+Inductive stack_step : state → prog * stack → prog * stack → Prop :=
+  | SS_Push : ∀st stk n p',
+    stack_step st (SPush n :: p', stk) (p', n :: stk)
+  | SS_Load : ∀st stk i p',
+    stack_step st (SLoad i :: p', stk) (p', st i :: stk)
+  | SS_Plus : ∀st stk n m p',
+    stack_step st (SPlus :: p', n::m::stk) (p', (m+n)::stk)
+  | SS_Minus : ∀st stk n m p',
+    stack_step st (SMinus :: p', n::m::stk) (p', (m-n)::stk)
+  | SS_Mult : ∀st stk n m p',
+    stack_step st (SMult :: p', n::m::stk) (p', (m*n)::stk).
+Theorem stack_step_deterministic : ∀st,
+  deterministic (stack_step st).
+Proof.
+  unfold deterministic. intros st x y1 y2 H1 H2.
+  induction H1; inversion H2; reflexivity.
+Qed.
+
+Definition stack_multistep st := multi (stack_step st).
+
+(* Leaving the correctness of compiler *)
+  
