Coq/Coq30.v
@@ -1,0 +1,11 @@
+(*
+  Exercies for <Software Foundations> V2 CH6.
+  Author : Brethland, Late 2019.
+*)
+
+Set Warnings "-notation-overridden,-parsing".
+From Coq Require Import Arith.Arith.
+Add LoadPath "C:\Users\ycy12\Documents\Workspace\LEARNING-STUFF\Coq".
+Load Coq29.
+Hint Constructors multi.
+
