Agda/Ag12.agda
@@ -5,38 +5,60 @@ open Eq
 open import Data.Nat using (ℕ; zero; suc; _+_; _*_)
 open import Relation.Nullary using (¬_)
 open import Data.Product using (_×_; proj₁; proj₂) renaming (_,_ to ⟨_,_⟩)
-open import Data.Sum using (_⊎_)
-open import Ag09
-open import Data.Product using (Σ; _,_; ∃; Σ-syntax; ∃-syntax)
+open import Data.Sum using (_⊎_; inj₁; inj₂)
+open import Function
+open import Ag09 hiding (_∘_)
+-- open import Data.Product using (Σ; _,_; ∃; Σ-syntax; ∃-syntax)
 open import Level using (Level; _⊔_) renaming (zero to lzero; suc to lsuc)
 open ≡-Reasoning
 open ≃-Reasoning
+
+postulate
+  funExt : ∀ {m n : Level} {A : Set m} {B : Set n} {f g : A → B}
+           → (∀ (x : A) → f x ≡ g x)
+           → f ≡ g
+
+lemma₀ : ∀ {A B : Set} → (a : A × B) → ⟨ proj₁ a , proj₂ a ⟩ ≡ a
+lemma₀ ⟨ fst , snd ⟩ = refl
+
+lemma₁ : ∀ {A : Set} {B C : A → Set}
+         → (f : (x : A) → B x × C x)
+         → (λ a → ⟨ proj₁ (f a) , proj₂ (f a) ⟩) ≡ f
+lemma₁ f = refl
 
 ∀-distrib-× : ∀ {A : Set} {B C : A → Set} →
   (∀ (x : A) → B x × C x) ≃ (∀ (x : A) → B x) × (∀ (x : A) → C x)
 ∀-distrib-× {A} {B} {C} =
   record
-  { to = λ x → ⟨ (λ x₁ → proj₁ (x x₁)) , (λ x₁ → proj₂ (x x₁)) ⟩
-  ; from = λ x y → ⟨ proj₁ x y , proj₂ x y ⟩
-  ; from∘to = λ x₁ → {!!}
-  ; to∘from = {!!}
+  { to      = λ bc → ⟨ proj₁ ∘ bc , proj₂ ∘ bc ⟩
+  ; from    = λ bc a → ⟨ proj₁ bc a , proj₂ bc a ⟩
+  ; from∘to = λ f → refl
+  ; to∘from = λ f → refl
   }
-
 ⊎∀-implies-∀⊎ : ∀ {A : Set} {B C : A → Set} →
   (∀ (x : A) → B x) ⊎ (∀ (x : A) → C x)  →  ∀ (x : A) → B x ⊎ C x
 ⊎∀-implies-∀⊎ (_⊎_.inj₁ x₁) x = _⊎_.inj₁ (x₁ x)
 ⊎∀-implies-∀⊎ (_⊎_.inj₂ y) x = _⊎_.inj₂ (y x)
 
-data Tri : Set where
-  aa : Tri
-  bb : Tri
-  cc : Tri
+data Σ (A : Set) (B : A → Set) : Set where
+  ⟨_,_⟩ : (x : A) → B x → Σ A B
 
-lemma : ∀ {B : Tri → Set} → (∀ (x : Tri) → B x) ≃ (B aa × B bb × B cc)
-lemma {B} =
+Σ-syntax = Σ
+infix 2 Σ-syntax
+syntax Σ-syntax A (λ x → B) = Σ[ x ∈ A ] B
+
+∃ : ∀ {A : Set} (B : A → Set) → Set
+∃ {A} B = Σ A B
+
+∃-syntax = ∃
+syntax ∃-syntax (λ x → B) = ∃[ x ] B
+
+∃-distrib-⊎ : ∀ {A : Set} {B C : A → Set} →
+  ∃[ x ] (B x ⊎ C x) ≃ (∃[ x ] B x) ⊎ (∃[ x ] C x)
+∃-distrib-⊎ =
   record
-  { to = λ z → ⟨ z aa , ⟨ z bb , z cc ⟩ ⟩
-  ; from = λ P → λ{ aa → proj₁ P ; bb → proj₁ (proj₂ P) ; cc → proj₂ (proj₂ P)}
-  ; from∘to = λ k → {!!}
-  ; to∘from = λ z → {!!}
+  { to = λ x → {!!}
+  ; from = λ{ (inj₁ x) → ⟨ {!!} , {!!} ⟩ ; (inj₂ x) → {!!} }
+  ; from∘to = {!!}
+  ; to∘from = {!!}
   }
