Agda/Ag13.agda
@@ -1,0 +1,61 @@
+module Ag13 where
+
+import Relation.Binary.PropositionalEquality as Eq
+open Eq using (_≡_; refl)
+open Eq.≡-Reasoning
+open import Data.Nat using (ℕ; zero; suc)
+open import Data.Product using (_×_) renaming (_,_ to ⟨_,_⟩)
+open import Data.Sum using (_⊎_; inj₁; inj₂)
+open import Relation.Nullary using (¬_)
+open import Relation.Nullary.Negation using ()
+  renaming (contradiction to ¬¬-intro)
+open import Data.Unit using (⊤; tt)
+open import Data.Empty using (⊥; ⊥-elim)
+open import Ag09 using (_⇔_)
+
+data Bool : Set where
+  true  : Bool
+  false : Bool
+
+T : Bool → Set
+T true   =  ⊤
+T false  =  ⊥
+
+T→≡ : ∀ (b : Bool) → T b → b ≡ true
+T→≡ true tt   =  refl
+T→≡ false ()
+
+≡→T : ∀ {b : Bool} → b ≡ true → T b
+≡→T refl  =  tt
+
+data Dec (A : Set) : Set where
+  yes :   A → Dec A
+  no  : ¬ A → Dec A
+
+infix 4 _≤_
+
+data _≤_ : ℕ → ℕ → Set where
+
+  z≤n : ∀ {n : ℕ}
+      --------
+    → zero ≤ n
+
+  s≤s : ∀ {m n : ℕ}
+    → m ≤ n
+      -------------
+    → suc m ≤ suc n
+
+¬s≤z : ∀ {m : ℕ} → ¬ (suc m ≤ zero)
+¬s≤z ()
+
+¬s≤s : ∀ {m n : ℕ} → ¬ (m ≤ n) → ¬ (suc m ≤ suc n)
+¬s≤s ¬m≤n (s≤s m≤n) = ¬m≤n m≤n
+
+_≤?_ : ∀ (m n : ℕ) → Dec (m ≤ n)
+zero  ≤? n                   =  yes z≤n
+suc m ≤? zero                =  no ¬s≤z
+suc m ≤? suc n with m ≤? n
+...               | yes m≤n  =  yes (s≤s m≤n)
+...               | no ¬m≤n  =  no (¬s≤s ¬m≤n)
+
+
